substitution lemmas for erased and par completed

src/FcEtt/ett_par.v
@@ -13,6 +13,7 @@ Require Export FcEtt.ett_ind.
 Require Export FcEtt.ext_context_fv.
 
 Require Import FcEtt.ext_wf.
+Require Import FcEtt.ett_erased.
 Import ext_wf.
 
 
@@ -23,26 +24,6 @@ Require Export FcEtt.toplevel.
 
 Require Export FcEtt.ett_value.
 
-
-Lemma rctx_uniq : forall W a R, erased_tm W a R -> uniq W.
-Proof. intros W a R H. induction H; eauto.
-        - pick fresh x. eapply uniq_app_2; eauto.
-        - pick fresh c; eauto.
-Qed.
-
-Lemma erased_app_rctx : forall W1 W2 W3 a R, uniq (W1 ++ W2 ++ W3) -> 
-                               erased_tm (W1 ++ W3) a R ->
-                               erased_tm (W1 ++ W2 ++ W3) a R.
-Proof. intros W1 W2 W3 a R U H. generalize dependent W2. 
-       dependent induction H; intros; eauto.
-        - eapply erased_a_Abs with (L := union L (dom (W1 ++ W2 ++ W3))).
-          intros. rewrite <- app_assoc.
-          eapply H0; eauto. simpl_env. auto.
-        - eapply erased_a_Pi with (L := union L (dom (W1 ++ W2 ++ W3))); eauto.
-          intros. rewrite <- app_assoc.
-          eapply H1; eauto. simpl_env. auto.
-        - econstructor; eauto.
-Qed.
 
 Lemma par_app_rctx : forall S D W1 W2 W3 a a' R, uniq (W1 ++ W2 ++ W3) ->
                      Par S D (W1 ++ W3) a a' R -> 
@@ -68,195 +49,15 @@ Qed.
 
 (* TODO: move these definitions to the OTT file. *)
 
-Inductive multipar S D W ( a : tm) (R : role) : tm -> Prop :=
-| mp_refl : multipar S D W a R a
-| mp_step : forall b c, Par S D W a b R -> multipar S D W b R c -> multipar S D W a R c.
+Inductive multipar S D W ( a : tm) : tm -> role -> Prop :=
+| mp_refl : forall R, erased_tm W a R -> multipar S D W a a R
+| mp_step : forall R b c, Par S D W a b R -> multipar S D W b c R -> 
+                                             multipar S D W a c R.
 
 Hint Constructors multipar.
 
-
-(* NOTE: we have a database 'erased' for proving that terms are erased. *)
-
-(* Tactics concerning erased terms. *)
-
-Ltac erased_pick_fresh x :=
-  match goal with
-    [ |- erased_tm ?s ?R ] =>
-    let v := match s with
-             | a_UAbs _ _ _ => erased_a_Abs
-             | a_Pi _ _ _ _ => erased_a_Pi
-             | a_CPi _ _   => erased_a_CPi
-             | a_UCAbs _   => erased_a_CAbs
-             end
-    in pick fresh x and apply v
-  end.
-
-Ltac erased_inversion :=
-  repeat match goal with
-  | [H : erased_tm (a_UAbs _ _ _) _ |- _ ] =>
-    inversion H; subst; clear H
-  | [H : erased_tm (a_App _ _ _ _) _ |- _ ] =>
-    inversion H; subst; clear H
-  | [H : erased_tm (a_Pi _ _ _ _) _ |- _ ] =>
-    inversion H; subst; clear H
-  | [H : erased_tm (a_CPi _ _) _ |- _ ] =>
-    inversion H; subst; clear H
-  | [H : erased_tm (a_UCAbs _ ) _ |- _ ] =>
-    inversion H; subst; clear H
-  | [H : erased_tm (a_CApp _ _) _ |- _ ] =>
-    inversion H; subst; clear H
-end.
-(*
-Ltac erased_case :=
-  let x := fresh in
-  let h0 := fresh in
-  erased_pick_fresh x; eauto using lc_erase;
-  match goal with
-    [ H : forall x, erased_tm (erase (open_tm_wrt_tm ?b (a_Var_f x)) ?R) ?R |- _ ] =>
-    move: (H x) => h0; rewrite <- open_tm_erase_tm in h0; eauto
-  | [ H : ∀ c, erased_tm (erase (open_tm_wrt_co ?b (g_Var_f c)) ?R) ?R |- _ ] =>
-    move: (H x) => h0; rewrite <- open_co_erase_tm2 with (g := (g_Var_f x)) in h0; auto
-  end.
-
-
-Lemma erased_tm_erase_mutual : forall R0,
-  (forall a, lc_tm a -> erased_tm (erase a R0) R0)
-  /\ (forall a, lc_brs a -> True)
-  /\ (forall a, lc_co a -> True)
-  /\ (forall phi, lc_constraint phi -> forall a b A R, phi = (Eq a b A R) ->
-                                         erased_tm (erase a R0) R0 /\ erased_tm (erase b R0) R0
-                                         /\ erased_tm (erase A R0) R0).
-
-Proof. intro.
-  apply lc_tm_lc_brs_lc_co_lc_constraint_mutind; intros; simpl; eauto.
-  all: try solve [ try (destruct rho); simpl; eauto].
-  all: try solve [erased_case].
-  - destruct R, R0; auto. simpl. constructor; auto. apply rep_nsub_nom.
-  - destruct phi. destruct (H _ _ _ _ eq_refl) as (h0 & h1 & h2). simpl.
-    erased_case.
-  - inversion H2. subst. tauto.
-    Unshelve. all:auto.
-Qed.
-
-Lemma erased_tm_erase : forall R a, lc_tm a -> erased_tm (erase a R) R.
-Proof.
-  intros.
-  destruct erased_tm_erase_mutual with R.
-  eauto.
-Qed.
-
-Hint Resolve erased_tm_erase : erased. Locate multipar.
-*)
-Inductive erased_sort (W : role_context) : sort -> Prop := 
-| erased_Tm : forall a R, erased_tm W a R -> erased_sort W (Tm a R)
-| erased_Co : forall a b A R, erased_tm W a R -> erased_tm W b R -> erased_tm W A R -> erased_sort W (Co (Eq a b A R)).
-
-(* Check Forall_forall FIXME:?? *)
-
-Inductive erased_context : role_context -> context -> Prop :=
- | nil_erased_ctx : erased_context nil nil
- | co_erased_ctx : forall W G c a b A R,
-                   erased_sort W (Co (Eq a b A R)) -> erased_context W G -> 
-                   erased_context W ([(c, (Co (Eq a b A R)))] ++ G)
- | tm_erased_ctx : forall W G x A R, erased_context W G ->
-                   erased_sort W (Tm A R) ->
-                   erased_context ([(x,R)] ++ W) ([(x, (Tm A R))] ++ G).
-
-Lemma dom_erased_ctx_rctx_le_ctx : forall W G, erased_context W G ->
-                                               dom W [<=] dom G.
-Proof. intros; induction H; simpl; fsetdec.
-Qed.
-
-Lemma uniq_erased_ctx_rctx : forall W G, erased_context W G -> uniq G
-                                          -> uniq W.
-Proof. intros. induction H; auto.
-       apply IHerased_context. eapply uniq_app_2; eauto.
-       inversion H0. apply IHerased_context in H4. constructor.
-       auto. apply dom_erased_ctx_rctx_le_ctx in H. fsetdec.
-Qed.
-
 Definition joins S D W a b R := exists c, erased_tm W a R /\ erased_tm W b R /\
-                               multipar S D W a R c /\ multipar S D W b R c.
-
-
-Lemma erased_lc : forall W a R, erased_tm W a R -> lc_tm a.
-intros; induction H; auto.
-Qed.
-
-Hint Resolve erased_lc : lc.
-
-Lemma subst_tm_erased : forall W1 x R1 W2 a R b, 
-               erased_tm (W1 ++ [(x,R1)] ++ W2) a R ->
-               erased_tm W2 b R1 -> 
-               erased_tm (W1 ++ W2) (tm_subst_tm_tm b x a) R.
-Proof.
-  intros W1 x R1 W2 a R b H1 H2. dependent induction H1; simpl; eauto.
-  - destruct (x0 == x); auto. 
-     + subst. assert (P:R = R1).
-       eapply binds_mid_eq; eauto. subst. replace W1 with (nil ++ W1); eauto.
-       rewrite app_assoc. eapply erased_app_rctx; simpl_env; eauto.
-     + econstructor. eapply uniq_remove_mid; eauto.
-       eapply binds_remove_mid; eauto.
-  - pick fresh y and apply erased_a_Abs.
-     assert(P : a_Var_f y = tm_subst_tm_tm b x (a_Var_f y)).
-     {rewrite tm_subst_tm_tm_fresh_eq; auto. }
-     rewrite P.
-     rewrite <- tm_subst_tm_tm_open_tm_wrt_tm; auto.
-     rewrite <- app_assoc. eapply H0; eauto. simpl_env. auto.
-     eapply erased_lc; eauto.
-  - pick fresh y and apply erased_a_Pi; eauto.
-     assert(P : a_Var_f y = tm_subst_tm_tm b x (a_Var_f y)).
-     {rewrite tm_subst_tm_tm_fresh_eq; auto. }
-     rewrite P.
-     rewrite <- tm_subst_tm_tm_open_tm_wrt_tm; auto.
-     rewrite <- app_assoc. eapply H0; eauto. simpl_env. auto.
-     eapply erased_lc; eauto.
-  - pick fresh c and apply erased_a_CPi; eauto.
-     assert(P : g_Var_f c = tm_subst_tm_co b x (g_Var_f c)).
-     {rewrite tm_subst_tm_co_fresh_eq; auto. }
-     rewrite P.
-     rewrite <- tm_subst_tm_tm_open_tm_wrt_co; auto.
-     eapply H0; eauto. eapply erased_lc; eauto.
-  - pick fresh c and apply erased_a_CAbs; eauto.
-     assert(P : g_Var_f c = tm_subst_tm_co b x (g_Var_f c)).
-     {rewrite tm_subst_tm_co_fresh_eq; auto. }
-     rewrite P.
-     rewrite <- tm_subst_tm_tm_open_tm_wrt_co; auto.
-     eapply H0; eauto. eapply erased_lc; eauto.
-Qed.
-
-
-Lemma subst_co_erased : forall W c g a R, lc_co g -> erased_tm W a R -> erased_tm W (co_subst_co_tm g c a) R.
-Proof.
-  intros W c g a R lc H. generalize dependent g.
-  induction H; intros; simpl; eauto.
-  - eapply erased_a_Abs with (L := L).
-     intros x0 H1.
-     assert(P : a_Var_f x0 = co_subst_co_tm g c (a_Var_f x0)).
-     {rewrite co_subst_co_tm_fresh_eq; auto. }
-     rewrite P.
-     rewrite <- co_subst_co_tm_open_tm_wrt_tm; auto.
-   - eapply erased_a_Pi with (L := L); eauto.
-     intros x0 H2.
-     assert(P : a_Var_f x0 = co_subst_co_tm g c (a_Var_f x0)).
-     {rewrite co_subst_co_tm_fresh_eq; auto. }
-     rewrite P.
-     rewrite <- co_subst_co_tm_open_tm_wrt_tm; auto.
-   - eapply erased_a_CPi with (L := union L (singleton c)); eauto.
-     intros c0 H4.
-     assert(P : g_Var_f c0 = co_subst_co_co g c (g_Var_f c0)).
-     {rewrite co_subst_co_co_fresh_eq; auto. } 
-     rewrite P.
-     rewrite <- co_subst_co_tm_open_tm_wrt_co; auto.
-   - eapply erased_a_CAbs with (L := union L (singleton c)); eauto.
-     intros c0 H4.
-     assert(P : g_Var_f c0 = co_subst_co_co g c (g_Var_f c0)).
-     {rewrite co_subst_co_co_fresh_eq; auto. } 
-     rewrite P.
-     rewrite <- co_subst_co_tm_open_tm_wrt_co; auto.
-Qed.
-
-Hint Resolve subst_tm_erased subst_co_erased : erased.
+                               multipar S D W a c R /\ multipar S D W b c R.
 
 Lemma Par_lc1 : forall G D W a a' R , Par G D W a a' R -> lc_tm a.
   intros.  induction H; auto. eapply erased_lc; eauto.
@@ -283,133 +84,6 @@ Qed.
 
 Hint Resolve Par_lc1 Par_lc2 : lc.
 
-Lemma typing_erased_mutual:
-    (forall G b A R, Typing G b A R -> erased_tm (ctx_to_rctx G) b R) /\
-    (forall G0 phi (H : PropWff G0 phi),
-        forall A B T R, phi = Eq A B T R -> erased_tm (ctx_to_rctx G0) A R /\ 
-        erased_tm (ctx_to_rctx G0) B R /\ erased_tm (ctx_to_rctx G0) T R) /\
-     (forall G0 D p1 p2 (H : Iso G0 D p1 p2), True ) /\
-     (forall G0 D A B T R (H : DefEq G0 D A B T R), True) /\
-     (forall G0 (H : Ctx G0), True).
-Proof. 
-  apply typing_wff_iso_defeq_mutual; intros; repeat split; split_hyp; subst; 
-  simpl; auto.
-  all : try solve [inversion H2; subst; auto].
-  all : try solve [econstructor; eauto].
-  - econstructor. apply ctx_to_rctx_uniq; eauto.
-  - econstructor. apply ctx_to_rctx_uniq; eauto. 
-    eapply ctx_to_rctx_binds_tm; eauto.
-  - econstructor; eauto. econstructor. apply ctx_to_rctx_uniq.
-    eapply Typing_Ctx; eauto.
-  - destruct phi.
-    apply (@erased_a_CPi L); try solve [apply (H0 a b A R0); auto]; auto;
-    pose H2 := H0 a b A R0 eq_refl; inversion H2 as [H21 [H22 H23]]; econstructor; eassumption.
-  - econstructor. apply ctx_to_rctx_uniq. auto.
-Qed.
-
-
-Lemma Typing_erased: forall G b A R, Typing G b A R -> 
-                                     erased_tm (ctx_to_rctx G) b R.
-Proof.
-  apply typing_erased_mutual.
-Qed.
-
-Hint Resolve Typing_erased : erased.
-(*
-
-Lemma typing_erased_type_mutual:
-    (forall G b A R, Typing G b A R -> erased_tm (ctx_to_rctx G) A R) /\
-    (forall G0 phi (H : PropWff G0 phi), True) /\
-     (forall G0 D p1 p2 (H : Iso G0 D p1 p2), True ) /\
-     (forall G0 D A B T R (H : DefEq G0 D A B T R), True) /\
-     (forall G0 (H : Ctx G0), erased_context (ctx_to_rctx G0) G0).
-Proof.
-  apply typing_wff_iso_defeq_mutual; intros; repeat split; split_hyp; subst; simpl; auto.
-  all: eauto using Typing_erased.
-    all: try solve [inversion H; pick fresh x;
-      rewrite (tm_subst_tm_tm_intro x); auto;
-        eapply subst_tm_erased;
-        eauto using Typing_erased].
-  - induction H. 
-     + inversion b.
-     + inversion b. inversion H1.
-       simpl in H1. apply IHerased_context; auto.
-       inversion c; auto.
-     + inversion b. 
-        * inversion H1; subst. inversion H0; subst.
-          assert (P : [(x,R)] = nil ++ [(x,R)]). { auto. }
-          rewrite P. rewrite app_assoc. apply erased_app_rctx; eauto.
-          apply Ctx_uniq in c. simpl_env. apply dom_erased_ctx_rctx_le_ctx in H.
-          inversion c. constructor. eapply rctx_uniq; eauto. fsetdec.
-        * assert (P : [(x0,R0)] = nil ++ [(x0,R0)]). { auto. }
-          rewrite P. rewrite app_assoc. apply erased_app_rctx; auto.
-          simpl_env. apply dom_erased_ctx_rctx_le_ctx in H.
-          inversion c. constructor. eapply rctx_uniq; eauto. fsetdec.
-          simpl_env. inversion c. apply IHerased_context; eauto.
-  - inversion H; subst. apply Typing_erased in t0.
-    pick fresh x. rewrite (tm_subst_tm_tm_intro x); auto.
-    replace (ctx_to_rctx G) with (nil ++ (ctx_to_rctx G)); auto.
-    eapply subst_tm_erased; eauto.
-  - inversion H; pick fresh x;
-      rewrite (co_subst_co_tm_intro x); auto.
-        eapply subst_co_erased;
-        eauto using Typing_erased.
-  - apply Forall_forall.
-    intros s h0. destruct s.
-    destruct h0. inversion H1. econstructor.
-    eauto using Typing_erased.
-    eapply Forall_forall in H; eauto. simpl in H. auto.
-  - apply Forall_forall.
-    intros s h0. destruct s. inversion p. subst.
-    destruct h0. inversion H4. econstructor;  eauto using Typing_erased.
-    eapply Forall_forall in H; eauto. simpl in H. auto.
-Qed.
-
-Lemma Typing_erased_type : forall G b A R, Typing G b A R -> erased_tm A.
-Proof. apply typing_erased_type_mutual. Qed.
-
-Hint Resolve Typing_erased_type : erased.
-*)
-Lemma toplevel_erased1 : forall W F a A R, binds F (Ax a A R) toplevel -> 
-                                           uniq W -> erased_tm W a R.
-Proof.
-  intros.
-  move: (toplevel_closed H) => h0.
-  replace W with (nil ++ W ++ nil).
-  apply erased_app_rctx. simpl_env; auto.
-  simpl_env. pose (P := Typing_erased h0). simpl in P.
-  auto. simpl_env. auto.
-Qed.
-(*
-Lemma toplevel_erased2 : forall F a A R, binds F (Ax a A R) toplevel -> erased_tm A.
-Proof.
-  intros.
-  move: (toplevel_closed H) => h0.
-  eauto with erased.
-Qed.
-
-Hint Resolve toplevel_erased1 toplevel_erased2 : erased.
-*)
-(*
-(* Introduce a hypothesis about an erased opened term. *)
-Ltac erased_body x Ea :=
-    match goal with
-      [ H4 : ∀ x : atom, x `notin` ?L0 → erased_tm (open_tm_wrt_tm ?a (a_Var_f x))
-                         |- _ ] =>
-      move: (H4 x ltac:(auto)) => Ea; clear H4
-    end.
-
-(* Move this to ett_ind? *)
-Ltac eta_eq y EQ :=
-   match goal with
-      [ H :
-          ∀ x : atom,
-            x `notin` ?L → open_tm_wrt_tm ?a (a_Var_f x) =
-                           a_App ?b ?rho _ _ |- _ ] =>
-   move: (H y ltac:(auto)) =>  EQ
-end.
-*)
-
 Lemma Par_erased_tm_fst : forall G D W a a' R, Par G D W a a' R -> 
                                                erased_tm W a R.
 Proof. intros G D W a a' R H. induction H; eauto.
@@ -419,57 +93,32 @@ Lemma Par_erased_tm_snd : forall G D W a a' R, Par G D W a a' R ->
                                                erased_tm W a' R.
 Proof. intros G D W a a' R H. induction H; eauto.
         - inversion IHPar1; subst. pick fresh x.
-          assert (Q : tm_subst_tm_tm b' x (a_Var_f x) = b').
-          { simpl; destruct (@eq_dec tmvar _ x x); try done. }
-          rewrite <- Q. assert (P : tm_subst_tm_tm b' x a' = a').
-          { eapply tm_subst_tm_tm_fresh_eq; eauto. }
-          rewrite <- P. rewrite <- tm_subst_tm_tm_open_tm_wrt_tm.
-          replace W with (W ++ nil); auto. eapply subst_tm_erased; eauto.
-          simpl_env. auto. eapply erased_lc; eauto.
+          erewrite tm_subst_tm_tm_intro; eauto.
+          replace W with (nil ++ W); auto. eapply subst_tm_erased; eauto.
         - inversion IHPar; subst. pick fresh c.
-          assert (Q : co_subst_co_co g_Triv c (g_Var_f c) = g_Triv).
-          { simpl; destruct (@eq_dec covar _ c c); try done. }
-          rewrite <- Q. assert (P : co_subst_co_tm g_Triv c a' = a').
-          { eapply co_subst_co_tm_fresh_eq; eauto. }
-          rewrite <- P. rewrite <- co_subst_co_tm_open_tm_wrt_co.
-          replace W with (W ++ nil); auto. eapply subst_co_erased; eauto.
-          simpl_env. auto. auto.
-        - admit.
+          erewrite co_subst_co_tm_intro; eauto.
+          replace W with (nil ++ W); auto. eapply subst_co_erased; eauto.
+        - eapply erased_sub. eapply toplevel_erased1; eauto. auto.
         - inversion IHPar1; eauto.
         - inversion IHPar; eauto.
-Admitted.
-(*
-Lemma Par_erased_tm : forall G D a a' R, Par G D a a' R -> erased_tm a -> erased_tm a'.
-Proof.
-  intros G D a a' R Ep Ea.  induction Ep; inversion Ea; subst; eauto 2.
-  all: try solve [ erased_pick_fresh x; auto ].
-  all: eauto.
-  - move: (IHEp1 ltac:(auto)); inversion 1;
-    pick fresh x;
-    rewrite (tm_subst_tm_tm_intro x); auto;
-    apply subst_tm_erased; auto.
-  - move: (IHEp ltac:(auto)); inversion 1;
-    pick fresh x;
-    rewrite (co_subst_co_tm_intro x); auto;
-    apply subst_co_erased; auto.
-  - eauto with erased.
-  - constructor. apply IHEp1 in H2. inversion H2; subst.
-    constructor. auto. constructor. eauto.
-  - constructor. constructor. apply IHEp in H0. inversion H0. auto.
 Qed.
 
-Hint Resolve Par_erased_tm : erased.
+Lemma Par_rctx_uniq : forall G D W a a' R, Par G D W a a' R -> uniq W.
+Proof. intros. eapply rctx_uniq. eapply Par_erased_tm_fst; eauto.
+Qed.
+
+Hint Resolve Par_erased_tm_fst Par_erased_tm_snd : erased.
 
 (* ------------------------------------------------------------- *)
 
-Lemma Par_sub: forall S D a a' R1 R2, Par S D a a' R1 -> SubRole R1 R2 ->
-                                      Par S D a a' R2.
-Proof. intros S D a a' R1 R2 H SR. generalize dependent R2.
-       induction H; intros; simpl; eauto.
+Lemma Par_sub: forall S D W a a' R1 R2, Par S D W a a' R1 -> SubRole R1 R2 ->
+                                      Par S D W a a' R2.
+Proof. intros S D W a a' R1 R2 H SR. generalize dependent R2.
+       induction H; intros; simpl; eauto. econstructor.
+       eapply erased_sub; eauto.
 Qed.
-*)
 
-Lemma subst1 : forall b S D W W' a a' R1 R2 x, Par S D W a a' R1 -> 
+Lemma subst1 : forall b S D W W' a a' R1 R2 x, Par S D W' a a' R1 -> 
                erased_tm (W ++ [(x,R1)] ++ W') b R2 ->
                Par S D (W ++ W') (tm_subst_tm_tm a x b) (tm_subst_tm_tm a' x b) R2.
 Proof.
@@ -479,59 +128,34 @@ Proof.
    - constructor. constructor. eapply uniq_remove_mid; eauto.
    - destruct (x0 == x); auto. 
      + subst. assert (P:R = R1).
-       eapply binds_mid_eq; eauto. subst. replace W' with (W' ++ nil); eauto.
-       eapply par_app_rctx. simpl_env. eapply uniq_remove_mid; eauto.
-       simpl_env; eauto. 
+       eapply binds_mid_eq; eauto. subst. replace W with (nil ++ W); eauto.
+       rewrite app_assoc. eapply par_app_rctx.
+       simpl_env. eapply uniq_remove_mid; eauto.
+       simpl_env; eauto. eapply Par_sub; eauto.
      + econstructor. econstructor. eapply uniq_remove_mid; eauto.
-       eapply binds_remove_mid; eauto.
-   - eapply Par_Abs with (L := union L (singleton x)).
+       eapply binds_remove_mid; eauto. auto.
+   - eapply Par_Abs with (L := union (singleton x) L).
      intros x0 H1.
-     assert(P : a_Var_f x0 = tm_subst_tm_tm a x (a_Var_f x0)).
-     {rewrite tm_subst_tm_tm_fresh_eq; auto. }
-     assert(Q : a_Var_f x0 = tm_subst_tm_tm a' x (a_Var_f x0)).
-     {rewrite tm_subst_tm_tm_fresh_eq; auto. }
-     rewrite P.
-     rewrite <- tm_subst_tm_tm_open_tm_wrt_tm; auto.
-     rewrite <- P. rewrite Q.
-     rewrite <- tm_subst_tm_tm_open_tm_wrt_tm; auto.
-     rewrite <- Q. simpl_env. eapply H0; eauto. simpl_env. auto.
+     rewrite tm_subst_tm_tm_open_tm_wrt_tm_var; auto 1.
+     rewrite tm_subst_tm_tm_open_tm_wrt_tm_var; auto 1.
+     rewrite <- app_assoc. eapply H0; eauto.
      eapply Par_lc2; eauto. eapply Par_lc1; eauto.
    - econstructor; eauto.
-   - eapply Par_Pi with (L := union L (singleton x)); eauto.
+   - eapply Par_Pi with (L := union (singleton x) L); eauto.
      intros x0 H1.
-     assert(P : a_Var_f x0 = tm_subst_tm_tm a x (a_Var_f x0)).
-     {rewrite tm_subst_tm_tm_fresh_eq; auto. }
-     assert(Q : a_Var_f x0 = tm_subst_tm_tm a' x (a_Var_f x0)).
-     {rewrite tm_subst_tm_tm_fresh_eq; auto. }
-     rewrite P.
-     rewrite <- tm_subst_tm_tm_open_tm_wrt_tm; auto.
-     rewrite <- P. rewrite Q.
-     rewrite <- tm_subst_tm_tm_open_tm_wrt_tm; auto.
-     rewrite <- Q. simpl_env. eapply H0; eauto. simpl_env. auto.
+     rewrite tm_subst_tm_tm_open_tm_wrt_tm_var; auto 1.
+     rewrite tm_subst_tm_tm_open_tm_wrt_tm_var; auto 1.
+     rewrite <- app_assoc. eapply H0; eauto.
      eapply Par_lc2; eauto. eapply Par_lc1; eauto.
    - eapply Par_CPi with (L := union L (singleton x)); eauto.
      intros c H1.
-     assert(P : g_Var_f c = tm_subst_tm_co a x (g_Var_f c)).
-     {rewrite tm_subst_tm_co_fresh_eq; auto. }
-     assert(Q : g_Var_f c = tm_subst_tm_co a' x (g_Var_f c)).
-     {rewrite tm_subst_tm_co_fresh_eq; auto. }
-     rewrite P.
-     rewrite <- tm_subst_tm_tm_open_tm_wrt_co; auto.
-     rewrite <- P. rewrite Q.
-     rewrite <- tm_subst_tm_tm_open_tm_wrt_co; auto.
-     rewrite <- Q. eapply H0; eauto.
+     rewrite tm_subst_tm_tm_open_tm_wrt_co_var; auto 1.
+     rewrite tm_subst_tm_tm_open_tm_wrt_co_var; auto 1. eapply H0; eauto.
      eapply Par_lc2; eauto. eapply Par_lc1; eauto.
    - eapply Par_CAbs with (L := union L (singleton x)); eauto.
      intros c H1.
-     assert(P : g_Var_f c = tm_subst_tm_co a x (g_Var_f c)).
-     {rewrite tm_subst_tm_co_fresh_eq; auto. }
-     assert(Q : g_Var_f c = tm_subst_tm_co a' x (g_Var_f c)).
-     {rewrite tm_subst_tm_co_fresh_eq; auto. }
-     rewrite P.
-     rewrite <- tm_subst_tm_tm_open_tm_wrt_co; auto.
-     rewrite <- P. rewrite Q.
-     rewrite <- tm_subst_tm_tm_open_tm_wrt_co; auto.
-     rewrite <- Q. eapply H0; eauto.
+     rewrite tm_subst_tm_tm_open_tm_wrt_co_var; auto 1.
+     rewrite tm_subst_tm_tm_open_tm_wrt_co_var; auto 1. eapply H0; eauto.
      eapply Par_lc2; eauto. eapply Par_lc1; eauto.
    - econstructor; eauto.
    - econstructor; eauto.
@@ -539,127 +163,163 @@ Proof.
    - econstructor; eauto.
 Qed.
 
-Lemma open1 : forall b S D a a' L, Par S D a a'
-  -> (forall x, x `notin` L -> erased_tm (open_tm_wrt_tm b (a_Var_f x)))
-  -> Par S D (open_tm_wrt_tm b a) (open_tm_wrt_tm b a').
+Lemma open1 : forall b S D W L a a' R, Par S D W a a' R
+  -> (forall x, x `notin` L -> erased_tm W (open_tm_wrt_tm b (a_Var_f x)) R)
+  -> Par S D W (open_tm_wrt_tm b a) (open_tm_wrt_tm b a') R.
 Proof.
   intros.
   pick fresh x.
   rewrite (tm_subst_tm_tm_intro x); auto.
   rewrite [(_ _ a')] (tm_subst_tm_tm_intro x); auto.
-  apply subst1; auto.
+  replace W with (nil ++ W); auto. eapply subst1; eauto.
+  apply erased_app_rctx; simpl_env.
+  constructor; auto. eapply Par_rctx_uniq; eauto.
+  auto.
 Qed.
-*)
 
-Lemma subst2 : forall S D b x, lc_tm b ->
-  forall a a' R, Par S D a a' R -> Par S D (tm_subst_tm_tm b x a) (tm_subst_tm_tm b x a') R.
+
+Lemma subst2 : forall b S D W W' a a' R R1 x, 
+          Par S D (W ++ [(x,R1)] ++ W') a a' R -> 
+          erased_tm W' b R1 ->
+          Par S D (W ++ W') (tm_subst_tm_tm b x a) (tm_subst_tm_tm b x a') R.
 Proof.
-  intros S D b x EB a a' R PAR.
-  induction PAR; simpl.
+  intros b S D W W' a a' R R1 x PAR E.
+  dependent induction PAR; simpl. 
   all: eauto using tm_subst_tm_tm_lc_tm.
-  all: autorewrite with subst_open; auto.
-  all: try solve [Par_pick_fresh y; autorewrite with subst_open_var; eauto].
-  - rewrite tm_subst_tm_tm_fresh_eq.
-    eapply Par_Axiom; eauto.
-    match goal with
-    | [H : binds ?c ?phi ?G |- _ ] =>
-      move:  (toplevel_closed H) => h0
-    end.
-    move: (Typing_context_fv h0) => ?. split_hyp.
-    simpl in *.
+  all: autorewrite with subst_open; eauto.
+  all: try eapply erased_lc; eauto.
+  - econstructor. eapply subst_tm_erased; eauto.
+  - eapply Par_Abs with (L := union L (singleton x)).
+    intros x0 H1.
+    rewrite tm_subst_tm_tm_open_tm_wrt_tm_var; auto 1.
+    rewrite tm_subst_tm_tm_open_tm_wrt_tm_var; auto 1.
+    rewrite <- app_assoc. eapply H0. auto. simpl_env; auto.
+    auto. eapply erased_lc; eauto. eapply erased_lc; eauto.
+  - eapply Par_Pi with (L := union L (singleton x)); eauto.
+    intros x0 H2.
+    rewrite tm_subst_tm_tm_open_tm_wrt_tm_var; auto 1.
+    rewrite tm_subst_tm_tm_open_tm_wrt_tm_var; auto 1.
+    rewrite <- app_assoc. eapply H0. auto. simpl_env; auto.
+    auto. eapply erased_lc; eauto. eapply erased_lc; eauto.
+  - eapply Par_CAbs with (L := union L (singleton x)).
+    intros x0 H1.
+    rewrite tm_subst_tm_tm_open_tm_wrt_co_var; auto 1.
+    rewrite tm_subst_tm_tm_open_tm_wrt_co_var; auto 1.
+    eapply H0. auto. eauto. auto.
+    eapply erased_lc; eauto. eapply erased_lc; eauto.
+  - eapply Par_CPi with (L := union L (singleton x)); eauto.
+    intros x0 H4.
+    rewrite tm_subst_tm_tm_open_tm_wrt_co_var; auto 1.
+    rewrite tm_subst_tm_tm_open_tm_wrt_co_var; auto 1.
+    eapply H0. auto. eauto. auto.
+    eapply erased_lc; eauto. eapply erased_lc; eauto.
+  - eapply Par_Axiom; eauto. 
+    rewrite tm_subst_tm_tm_fresh_eq. eauto.
+    apply toplevel_closed in H.
+    apply Typing_context_fv in H.
+    split_hyp. simpl in *.
     fsetdec.
+  - pose (P := IHPAR _ _ _ _ ltac:(auto) E). simpl in P. auto.
+  - econstructor; eauto 2. pose (P := IHPAR1 _ _ _ _ ltac:(auto) E).
+    simpl in P. auto.
+  - econstructor; eauto. pose (P := IHPAR _ _ _ _ ltac:(auto) E).
+    simpl in P. auto.
 Qed.
 
-(*
-Lemma subst3 : forall S D b b' x R,
-    Par S D b b' R ->
-    forall a a', erased_tm a R -> Par S D a a' R ->
-    Par S D (tm_subst_tm_tm b x a) (tm_subst_tm_tm b' x a') R.
+
+Lemma subst3 : forall b b' S D W W' a a' R R1 x, 
+          Par S D (W ++ [(x,R1)] ++ W') a a' R -> 
+          Par S D W' b b' R1 ->
+          Par S D (W ++ W') (tm_subst_tm_tm b x a) (tm_subst_tm_tm b' x a') R.
 Proof.
   intros.
-  dependent induction H1; simpl; eauto 2; erased_inversion; eauto 4.
+  dependent induction H; simpl; eauto 2; erased_inversion; eauto 4.
   all: try solve [ Par_pick_fresh y;
               autorewrite with subst_open_var; eauto 3 with lc ].
   all: try solve [ autorewrite with subst_open; eauto 4 with lc ].
-  - apply subst1; auto.
+  - eapply subst1; eauto.
+  - eapply Par_Abs with (L := union L (singleton x)).
+    intros x0 H2.
+    rewrite tm_subst_tm_tm_open_tm_wrt_tm_var; auto 1.
+    rewrite tm_subst_tm_tm_open_tm_wrt_tm_var; auto 1.
+    rewrite <- app_assoc. eapply H0. auto. simpl_env; auto.
+    auto. eapply Par_lc2; eauto. eapply Par_lc1; eauto.
+  - eapply Par_Pi with (L := union (singleton x) L); eauto.
+    intros x0 H3.
+    rewrite tm_subst_tm_tm_open_tm_wrt_tm_var; auto 1.
+    rewrite tm_subst_tm_tm_open_tm_wrt_tm_var; auto 1.
+    rewrite <- app_assoc. eapply H1; eauto. simpl_env; auto.
+    eapply Par_lc2; eauto. eapply Par_lc1; eauto.
   - eapply Par_Axiom; eauto.
     rewrite tm_subst_tm_tm_fresh_eq. eauto.
-    match goal with
-    | [H : binds ?c ?phi ?G |- _ ] =>
-      move:  (toplevel_closed H) => h0
-    end.
-     move: (Typing_context_fv h0) => ?. split_hyp.
-     fsetdec. 
+    apply toplevel_closed in H.
+    apply Typing_context_fv in H.
+    split_hyp. simpl in *.
+    fsetdec.
+  - pose (P := IHPar _ _ _ _ ltac:(auto) H0). simpl in P. auto.
+  - econstructor; eauto 2. pose (P := IHPar1 _ _ _ _ ltac:(auto) H1).
+    simpl in P. auto.
+  - econstructor; eauto. pose (P := IHPar _ _ _ _ ltac:(auto) H0).
+    simpl in P. auto.
 Qed.
-*)
 
 Lemma subst4 : forall S D b x, lc_co b ->
-    forall a a' R, Par S D a a' R ->
-    Par S D (co_subst_co_tm b x a) (co_subst_co_tm b x a') R.
+    forall W a a' R, Par S D W a a' R ->
+    Par S D W (co_subst_co_tm b x a) (co_subst_co_tm b x a') R.
 Proof.
-  intros S D b x EB a a' R PAR.
+  intros S D b x EB W a a' R PAR.
   induction PAR; simpl; auto.
   all: try solve [ Par_pick_fresh y;
               autorewrite with subst_open_var; eauto 3 with lc ].
   all: try solve [ autorewrite with subst_open; eauto 4 with lc ].
-  - apply Par_Refl. eapply co_subst_co_tm_lc_tm; auto.
+  - apply Par_Refl. eapply subst_co_erased; eauto.
   - rewrite co_subst_co_tm_fresh_eq. eauto.
-    match goal with
-    | [H : binds ?c ?phi ?G |- _ ] =>
-      move:  (toplevel_closed H) => h0
-    end.
-    move: (Typing_context_fv  h0) => ?. split_hyp.
-    simpl in *.
+    apply toplevel_closed in H.
+    apply Typing_context_fv in H.
+    split_hyp. simpl in *.
     fsetdec.
 Qed.
-(*
-Lemma multipar_subst3 : forall S D b b' x R, erased_tm b R ->
-    multipar S D b b' R ->
-    forall a a', erased_tm a R -> multipar S D a a' R ->
-    multipar S D (tm_subst_tm_tm b x a) (tm_subst_tm_tm b' x a') R.
+
+Lemma multipar_subst3 : forall b b' S D W W' a a' R R1 x, 
+     multipar S D (W ++ [(x,R1)] ++ W') a a' R -> 
+     multipar S D W' b b' R1 ->
+     multipar S D (W ++ W') (tm_subst_tm_tm b x a) (tm_subst_tm_tm b' x a') R.
 Proof.
-  intros S D b b' x R lc H.
-  dependent induction H; auto.
-  - intros a0 a' lc2 H.
-    dependent induction H; auto.
-    apply (@mp_step _ _ _ _ ((tm_subst_tm_tm a x b))); auto.
-    apply subst3; auto.
-    apply Par_Refl; eapply erased_lc; eauto.
-    apply IHmultipar.
-    eapply Par_erased_tm; eauto.
-  - intros a0 a' lc2 H1.
-    dependent induction H1; auto.
-    apply (@mp_step _ _ _ _ (tm_subst_tm_tm b x a0)); auto.
-    apply subst3; auto.
-    apply Par_Refl; eapply erased_lc; eauto.
+  intros b b' S D W W' a a' R R1 x H1 H2.
+  dependent induction H1; auto.
+  - dependent induction H2; auto.
+    constructor. eapply subst_tm_erased; eauto.
+    apply (@mp_step _ _ _ _ _ ((tm_subst_tm_tm b x a))); auto.
+    eapply subst3; eauto.
+  - dependent induction H2; auto.
+    apply (@mp_step _ _ _ _ _ (tm_subst_tm_tm a0 x b0)); auto.
+    eapply subst3; eauto.
+    apply (@mp_step _ _ _ _ _ ((tm_subst_tm_tm a0 x b0))); auto.
+    eapply subst2; eauto. eapply Par_erased_tm_fst; eauto.
     apply IHmultipar; auto.
-    eapply Par_erased_tm; eauto.
-    apply (@mp_step _ _ _ _ ((tm_subst_tm_tm a x b0))); auto.
-    apply subst2; auto.
-    eapply Par_lc1; eauto.
-    apply IHmultipar0; auto.
-    eapply Par_erased_tm; eauto.
+    econstructor; eauto.
 Qed.
-*)
-Lemma multipar_subst4 : forall S D b x, lc_co b ->
-    forall a a' R, multipar S D a a' R ->
-    multipar S D (co_subst_co_tm b x a) (co_subst_co_tm b x a') R.
+
+Lemma multipar_subst4 : forall S D W b x, lc_co b ->
+    forall a a' R, multipar S D W a a' R ->
+    multipar S D W (co_subst_co_tm b x a) (co_subst_co_tm b x a') R.
 Proof.
-  intros S D b x H a a' R H0.
+  intros S D W b x H a a' R H0.
   dependent induction H0; eauto.
-  apply (@mp_step _ _ _ R (co_subst_co_tm b x b0)); auto.
+  constructor. eapply subst_co_erased; eauto.
+  apply (@mp_step _ _ _ _ _ (co_subst_co_tm b x b0)); auto.
   apply subst4; auto.
 Qed.
-(*
-Lemma erased_tm_open_tm_wrt_tm: forall a x, erased_tm a -> erased_tm (open_tm_wrt_tm a (a_Var_f x)).
+
+Lemma erased_tm_open_tm_wrt_tm: forall W a R x, erased_tm W a R -> erased_tm W (open_tm_wrt_tm a (a_Var_f x)) R.
 Proof.
-  intros a x H.
+  intros W a R x H.
   pose K := erased_lc H.
   rewrite open_tm_wrt_tm_lc_tm; eauto.
 Qed.
 
 Hint Resolve erased_tm_open_tm_wrt_tm : erased.
-*)
+
 
 Lemma Par_Pi_exists: ∀ x (G : context) D rho (A B A' B' : tm) R R',
     x `notin` fv_tm_tm_tm B -> Par G D A A' R
